<?xml version="1.0"?>


<!DOCTYPE rdf:RDF [
    <!ENTITY owl "http://www.w3.org/2002/07/owl#" >
    <!ENTITY xsd "http://www.w3.org/2001/XMLSchema#" >
    <!ENTITY rdfs "http://www.w3.org/2000/01/rdf-schema#" >
    <!ENTITY rdf "http://www.w3.org/1999/02/22-rdf-syntax-ns#" >
    <!ENTITY ProcurementsTopClasses "https://loted2.googlecode.com/svn/trunk/modules/ProcurementsTopClasses#" >
    <!ENTITY SubjectiveLegalSituationsInProcurements "https://loted2.googlecode.com/svn/trunk/modules/SubjectiveLegalSituationsInProcurements#" >
    <!ENTITY ProcurementSubjectiveScope "https://loted2.googlecode.com/svn/trunk/modules/ProcurementSubjectiveScope#" >
    <!ENTITY BusinessEntity "https://loted2.googlecode.com/svn/trunk/modules/BusinessEntity#">
    <!ENTITY TenderDocuments "https://loted2.googlecode.com/svn/trunk/modules/TenderDocuments#" >
    <!ENTITY ProcurementCompetitiveProcess "https://loted2.googlecode.com/svn/trunk/modules/ProcurementCompetitiveProcess#" >
    <!ENTITY TenderBid "https://loted2.googlecode.com/svn/trunk/modules/TenderBid#" >

]>


<rdf:RDF xmlns="https://loted2.googlecode.com/svn/trunk/modules/SubjectiveLegalSituationsInProcurements#"
     xml:base="https://loted2.googlecode.com/svn/trunk/modules/SubjectiveLegalSituationsInProcurements"
     xmlns:rdfs="http://www.w3.org/2000/01/rdf-schema#"
     xmlns:ProcurementsTopClasses="https://loted2.googlecode.com/svn/trunk/modules/ProcurementsTopClasses#"
     xmlns:ProcurementSubjectiveScope="https://loted2.googlecode.com/svn/trunk/modules/ProcurementSubjectiveScope#"
     xmlns:BusinessEntity="https://loted2.googlecode.com/svn/trunk/modules/BusinessEntity#"
     xmlns:TenderDocuments="https://loted2.googlecode.com/svn/trunk/modules/TenderDocuments#"
     xmlns:TenderBid="https://loted2.googlecode.com/svn/trunk/modules/TenderBid#"
     xmlns:ProcurementCompetitiveProcess="https://loted2.googlecode.com/svn/trunk/modules/ProcurementCompetitiveProcess#"
     xmlns:owl="http://www.w3.org/2002/07/owl#"
     xmlns:xsd="http://www.w3.org/2001/XMLSchema#"
     xmlns:rdf="http://www.w3.org/1999/02/22-rdf-syntax-ns#"
     xmlns:dc="http://purl.org/dc/terms/">
    <owl:Ontology rdf:about="https://loted2.googlecode.com/svn/trunk/modules/SubjectiveLegalSituationsInProcurements">
        <owl:versionIRI rdf:resource="https://loted2.googlecode.com/svn/trunk/modules/SubjectiveLegalSituationsInProcurements"/>
        		<!-- dc: metadata for documentation LODE -->
		<dc:creator>Isabella Distinto</dc:creator>
        <rdfs:label xml:lang="en">Subjective legal situations in procurements</rdfs:label>
        <owl:versionInfo xml:lang="en">2.0</owl:versionInfo>
		<rdfs:comment xml:lang="en">The Subjective Legal Situations module, which is part of the LOTED2 ontology, describes the types of roles played by the agents in the context of a procurement competitive process.</rdfs:comment>
        <dc:title rdf:datatype="&xsd;string">LOTED2: Subjective Legal Situations Module</dc:title>
        <dc:contributor rdf:datatype="&xsd;string">Enrico Motta</dc:contributor>
        <dc:contributor rdf:datatype="&xsd;string">Mathieu d'Aquin</dc:contributor>
		<dc:description rdf:datatype="&xsd;string">The ontology was created by Isabella Distinto, with input from Mathieu d'Aquin and Enrico Motta.</dc:description>
        <dc:language rdf:datatype="&xsd;language">en</dc:language>
        <dc:date>2013-07-24</dc:date>
       <!-- dc: metadata end -->    
    </owl:Ontology>
    


    <!-- 
    ///////////////////////////////////////////////////////////////////////////////////////
    //
    // Annotation properties
    //
    ///////////////////////////////////////////////////////////////////////////////////////
     -->

    


    <!-- 
    ///////////////////////////////////////////////////////////////////////////////////////
    //
    // Datatypes
    //
    ///////////////////////////////////////////////////////////////////////////////////////
     -->

    


    <!-- 
    ///////////////////////////////////////////////////////////////////////////////////////
    //
    // Object Properties
    //
    ///////////////////////////////////////////////////////////////////////////////////////
     -->

    


    <!-- https://loted2.googlecode.com/svn/trunk/modules/ProcurementsTopClasses#playsRole -->

    <rdf:Description rdf:about="&ProcurementsTopClasses;playsRole">
        <owl:propertyChainAxiom rdf:parseType="Collection">
            <rdf:Description rdf:about="&SubjectiveLegalSituationsInProcurements;hasLegalSituation"/>
            <rdf:Description rdf:about="&SubjectiveLegalSituationsInProcurements;role"/>
        </owl:propertyChainAxiom>
    </rdf:Description>
   

    <!-- &SubjectiveLegalSituationsInProcurements;hasLegalSituation -->

    <owl:ObjectProperty rdf:about="&SubjectiveLegalSituationsInProcurements;hasLegalSituation">
        <rdfs:label xml:lang="en">hasLegalSituation (0..*)</rdfs:label>
        <rdfs:comment xml:lang="en">A natural or legal person may have one or more legal situation in one or more contexts</rdfs:comment>
        <rdfs:range rdf:resource="&SubjectiveLegalSituationsInProcurements;SubjectiveLegalSituation"/>
        <owl:inverseOf rdf:resource="&SubjectiveLegalSituationsInProcurements;isLegalSituationOf"/>
        <rdfs:domain>
            <owl:Class>
                <owl:unionOf rdf:parseType="Collection">
                    <rdf:Description rdf:about="&ProcurementsTopClasses;LegalPerson"/>
                    <rdf:Description rdf:about="&ProcurementsTopClasses;NaturalPerson"/>
                </owl:unionOf>
            </owl:Class>
        </rdfs:domain>
    </owl:ObjectProperty>
    


    <!-- &SubjectiveLegalSituationsInProcurements;inOrFor -->

    <owl:ObjectProperty rdf:about="&SubjectiveLegalSituationsInProcurements;inOrFor">
        <rdfs:label xml:lang="en">in or for (1..1)</rdfs:label>
        <rdfs:comment xml:lang="en">The subjective legal situation is referred to a context (process), in which the natural or legal person plays a role</rdfs:comment>
        <rdfs:range rdf:resource="&ProcurementsTopClasses;Process"/>
        <rdfs:domain rdf:resource="&SubjectiveLegalSituationsInProcurements;SubjectiveLegalSituation"/>
    </owl:ObjectProperty>
    


    <!-- &SubjectiveLegalSituationsInProcurements;isLegalSituationOf -->

    <owl:ObjectProperty rdf:about="&SubjectiveLegalSituationsInProcurements;isLegalSituationOf">
        <rdfs:label xml:lang="en">is legal situation of</rdfs:label>
    </owl:ObjectProperty>
    


    <!-- &SubjectiveLegalSituationsInProcurements;role -->

    <owl:ObjectProperty rdf:about="&SubjectiveLegalSituationsInProcurements;role">
        <rdfs:label xml:lang="en">role (0..1)</rdfs:label>
        <rdfs:comment xml:lang="en">Th role that characterizes the subjective legal situation</rdfs:comment>
        <rdfs:range rdf:resource="&ProcurementsTopClasses;LegalRole"/>
        <rdfs:domain rdf:resource="&SubjectiveLegalSituationsInProcurements;SubjectiveLegalSituation"/>
    </owl:ObjectProperty>
    


    <!-- 
    ///////////////////////////////////////////////////////////////////////////////////////
    //
    // Classes
    //
    ///////////////////////////////////////////////////////////////////////////////////////
     -->

    


    <!-- &SubjectiveLegalSituationsInProcurements;AwardingLegalEntity -->

    <owl:Class rdf:about="&SubjectiveLegalSituationsInProcurements;AwardingLegalEntity">
        <rdfs:label xml:lang="en">Awarding legal entity</rdfs:label>
        <rdfs:subClassOf rdf:resource="&SubjectiveLegalSituationsInProcurements;RoleInProcurement"/>
        <rdfs:comment xml:lang="en">Any legal entity which has the role of awarding entity. 

This is a general class which comprises both the contracting authority and the contracting entity role.</rdfs:comment>
    </owl:Class>
    


    <!-- &SubjectiveLegalSituationsInProcurements;Candidate -->

    <owl:Class rdf:about="&SubjectiveLegalSituationsInProcurements;Candidate">
        <rdfs:label xml:lang="en">Candidate</rdfs:label>
        <rdfs:subClassOf rdf:resource="&SubjectiveLegalSituationsInProcurements;EconomicOperator"/>
        <rdfs:comment xml:lang="en">A candidate is any natural or legal person acting in the market as economic operator (i.e. a BusinessEntity) which has sought an invitation to take part in a restricted or negotiated procedure or in a competitive dialogue.</rdfs:comment>
<owl:equivalentClass>
			<owl:Class>
				<owl:intersectionOf rdf:parseType="Collection">
					<rdf:Description rdf:about="&SubjectiveLegalSituationsInProcurements;RoleInProcurement"/>
					<owl:Restriction>
						<owl:onProperty rdf:resource="&ProcurementsTopClasses;rolePlayedBy"/>
						<owl:allValuesFrom>
							<owl:Class>
								<owl:intersectionOf rdf:parseType="Collection">
									<owl:Class>
										<owl:unionOf rdf:parseType="Collection">
											<rdf:Description rdf:about="&ProcurementsTopClasses;LegalPerson"/>
											<rdf:Description rdf:about="&ProcurementsTopClasses;NaturalPerson"/>
										</owl:unionOf>
									</owl:Class>
									<owl:Restriction>
										<owl:onProperty rdf:resource="&TenderDocuments;hasSought"/>
										<owl:someValuesFrom rdf:resource="&TenderDocuments;InvitationToSubmitATender"/>
									</owl:Restriction>
								</owl:intersectionOf>
							</owl:Class>
						</owl:allValuesFrom>
					</owl:Restriction>
				</owl:intersectionOf>
			</owl:Class>
		</owl:equivalentClass>
    </owl:Class>
    


    <!-- &SubjectiveLegalSituationsInProcurements;ContractingAuthority -->

    <owl:Class rdf:about="&SubjectiveLegalSituationsInProcurements;ContractingAuthority">
        <rdfs:label xml:lang="en">Contracting authority</rdfs:label>
        <rdfs:subClassOf rdf:resource="&SubjectiveLegalSituationsInProcurements;AwardingLegalEntity"/>
        <rdfs:comment xml:lang="en">&quot;Contracting authorities&quot; means the role played by entity operating in ordinary sectors in the context of any procurement competitive process.

For example: The body governed by public law X issues a contract notice Y through which is announced the tender Z for the award of contract J, then the body governed by public law X plays the role of contracting authority in the context Z</rdfs:comment>
<owl:equivalentClass>
			<owl:Class>
				<owl:intersectionOf rdf:parseType="Collection">
					<rdf:Description rdf:about="&SubjectiveLegalSituationsInProcurements;RoleInProcurement"/>
					<owl:Restriction>
						<owl:onProperty rdf:resource="&ProcurementsTopClasses;rolePlayedBy"/>
						<owl:allValuesFrom rdf:resource="&ProcurementSubjectiveScope;EntityOperatingInOrdinarySectors"/>
					</owl:Restriction>
				</owl:intersectionOf>
			</owl:Class>
		</owl:equivalentClass>
    </owl:Class>
    


    <!-- &SubjectiveLegalSituationsInProcurements;ContractingEntity -->

    <owl:Class rdf:about="&SubjectiveLegalSituationsInProcurements;ContractingEntity">
        <rdfs:label xml:lang="en">Contracting entity</rdfs:label>
        <rdfs:subClassOf rdf:resource="&SubjectiveLegalSituationsInProcurements;AwardingLegalEntity"/>
        <rdfs:comment xml:lang="en">&quot;Contracting entity&quot; means the role played by an entity operating in utilities in the context of any procurement competitive process.</rdfs:comment>
<owl:equivalentClass>
			<owl:Class>
				<owl:intersectionOf rdf:parseType="Collection">
					<rdf:Description rdf:about="&SubjectiveLegalSituationsInProcurements;RoleInProcurement"/>
					<owl:Restriction>
						<owl:onProperty rdf:resource="&ProcurementsTopClasses;rolePlayedBy"/>
						<owl:allValuesFrom rdf:resource="&ProcurementSubjectiveScope;EntityOperatingInUtilities"/>
					</owl:Restriction>
				</owl:intersectionOf>
			</owl:Class>
		</owl:equivalentClass>
    </owl:Class>
    


    <!-- &SubjectiveLegalSituationsInProcurements;EconomicOperator -->

    <owl:Class rdf:about="&SubjectiveLegalSituationsInProcurements;EconomicOperator">
        <rdfs:label xml:lang="en">Economic operator</rdfs:label>
        <rdfs:subClassOf rdf:resource="&SubjectiveLegalSituationsInProcurements;RoleInProcurement"/>
        <rdfs:comment xml:lang="en">The EU procurements Directives define the term &quot;economic operator&quot; as the term that covers equally the concepts of &quot;contractor&quot;, &quot;supplier&quot; and &quot;service provider&quot;.  Each of these terms mean any natural or legal person or public entity or group of such persons and/or bodies which offers on the market, respectively, the execution of works and/or a work, products or services.

Thus, in the context of European public procurements, we can argue that &quot;Economic operator&quot; is the role played by any natural or legal person that offers in the market some gr:Offering.</rdfs:comment>
    </owl:Class>
    


    <!-- &SubjectiveLegalSituationsInProcurements;EligibleEconomicOperator -->

    <owl:Class rdf:about="&SubjectiveLegalSituationsInProcurements;EligibleEconomicOperator">
        <rdfs:label xml:lang="en">Eligible economic operator</rdfs:label>
        <rdfs:subClassOf rdf:resource="&SubjectiveLegalSituationsInProcurements;EconomicOperator"/>
        <rdfs:comment xml:lang="en">Any agent that plays the role of economic operator in the market and satisfies the eligibility criteria for participating in public contracts (artt. 45-50 Directive 2004/18/ec), as for example the absence of conviction by final judgement for participation in criminal organisation, fraud, corruption, money laundering, etc.</rdfs:comment>
    </owl:Class>
    


    <!-- &SubjectiveLegalSituationsInProcurements;PublicWorksConcessionaire -->

    <owl:Class rdf:about="&SubjectiveLegalSituationsInProcurements;PublicWorksConcessionaire">
        <rdfs:label xml:lang="en">Public works concessionaire</rdfs:label>
        <rdfs:subClassOf rdf:resource="&SubjectiveLegalSituationsInProcurements;EconomicOperator"/>
        <rdfs:comment xml:lang="en">When a public works concessionaire intends to award a contract to a third party, it has to make known its intention through a contract notice, either if is a public authority or a private legal person. Thus, a legal person who plays the role of public works concessionaire is empowered to issue contract notices for the award of works public contracts.</rdfs:comment>
    </owl:Class>
    


    <!-- &SubjectiveLegalSituationsInProcurements;QualifiedEconomicOperator -->

    <owl:Class rdf:about="&SubjectiveLegalSituationsInProcurements;QualifiedEconomicOperator">
        <rdfs:label xml:lang="en">Qualified economic operator</rdfs:label>
        <rdfs:subClassOf rdf:resource="&SubjectiveLegalSituationsInProcurements;EconomicOperator"/>
        <rdfs:comment xml:lang="en">Any economic operator that has been recognized as qualified for a given contract through a qualification system</rdfs:comment>
    </owl:Class>
    


    <!-- &SubjectiveLegalSituationsInProcurements;RoleInProcurement -->

    <owl:Class rdf:about="&SubjectiveLegalSituationsInProcurements;RoleInProcurement">
        <rdfs:label xml:lang="en">Role in procurement</rdfs:label>
        <rdfs:subClassOf rdf:resource="&ProcurementsTopClasses;LegalRole"/>
        <owl:disjointWith rdf:resource="&SubjectiveLegalSituationsInProcurements;SubjectiveLegalSituation"/>
        <rdfs:comment xml:lang="en">This is the class of any type of role played in procurement competitive processes</rdfs:comment>
<owl:equivalentClass>
			<owl:Class>
				<owl:intersectionOf rdf:parseType="Collection">
					<rdf:Description rdf:about="&ProcurementsTopClasses;LegalRole"/>
					<owl:Restriction>
						<owl:onProperty rdf:resource="&ProcurementsTopClasses;context"/>
						<owl:allValuesFrom rdf:resource="&ProcurementCompetitiveProcess;ProcurementCompetitiveProcess"/>
					</owl:Restriction>
				</owl:intersectionOf>
			</owl:Class>
		</owl:equivalentClass>
    </owl:Class>
    


    <!-- &SubjectiveLegalSituationsInProcurements;ServiceConcessionaire -->

    <owl:Class rdf:about="&SubjectiveLegalSituationsInProcurements;ServiceConcessionaire">
        <rdfs:label xml:lang="en">Service concessionaire</rdfs:label>
        <rdfs:subClassOf rdf:resource="&SubjectiveLegalSituationsInProcurements;EconomicOperator"/>
    </owl:Class>
    


    <!-- &SubjectiveLegalSituationsInProcurements;SubjectiveLegalSituation -->

    <owl:Class rdf:about="&SubjectiveLegalSituationsInProcurements;SubjectiveLegalSituation">
        <rdfs:label xml:lang="en">Subjective legal situation</rdfs:label>
        <rdfs:comment xml:lang="en">A subjective legl situation is any position held by a natural or legal person, characterized by a role played in a given context. 

A person may have one or more subjective legal situations.
For example a body governed by public law may have the position of contracting authority in the tender X, but may have the position of tenderer in the tender Y.</rdfs:comment>
    </owl:Class>
    


    <!-- &SubjectiveLegalSituationsInProcurements;Tenderer -->

    <owl:Class rdf:about="&SubjectiveLegalSituationsInProcurements;Tenderer">
        <rdfs:label xml:lang="en">Tenderer</rdfs:label>
        <rdfs:subClassOf rdf:resource="&SubjectiveLegalSituationsInProcurements;EconomicOperator"/>
        <rdfs:comment xml:lang="en">Any natural or legal person which plays the role of economic operator in the market and has submitted a tender bid for a public contract</rdfs:comment>
<owl:equivalentClass>
			<owl:Class>
				<owl:intersectionOf rdf:parseType="Collection">
					<rdf:Description rdf:about="&SubjectiveLegalSituationsInProcurements;RoleInProcurement"/>
					<owl:Restriction>
						<owl:onProperty rdf:resource="&ProcurementsTopClasses;rolePlayedBy"/>
						<owl:allValuesFrom>
							<owl:Class>
								<owl:intersectionOf rdf:parseType="Collection">
									<owl:Class>
										<owl:unionOf rdf:parseType="Collection">
											<rdf:Description rdf:about="&ProcurementsTopClasses;LegalPerson"/>
											<rdf:Description rdf:about="&ProcurementsTopClasses;NaturalPerson"/>
										</owl:unionOf>
									</owl:Class>
									<owl:Restriction>
										<owl:onProperty rdf:resource="&TenderBid;hasSubmitted"/>
										<owl:someValuesFrom rdf:resource="&TenderBid;TenderBid"/>
									</owl:Restriction>
								</owl:intersectionOf>
							</owl:Class>
						</owl:allValuesFrom>
					</owl:Restriction>
				</owl:intersectionOf>
			</owl:Class>
		</owl:equivalentClass>
    </owl:Class>
</rdf:RDF>



<!-- Generated by the OWL API (version 3.2.3.1824) http://owlapi.sourceforge.net -->

